Phi_System/IDE_CP_Core.thy
@@ -514,7 +514,6 @@ lemma [\<phi>reason %\<phi>programming_method]:
 end
 
 
-
 subsection \<open>Automation\<close>
 
 named_theorems \<phi>sledgehammer_simps \<open>Simplification rules used before applying slegehammer automation\<close>
@@ -2553,7 +2552,8 @@ setup \<open>Context.theory_map (
            not (can \<^keyword>\<open>certified\<close> (#toks arg))
         then let val id = Option.map (Phi_ID.encode o Phi_ID.cons (#id arg)) (Phi_ID.get_if_is_named ctxt)
                  val sequent' = Phi_Reasoners.obligation_intro_Ex_conv ~1 ctxt sequent
-              in raise Phi_CP_IDE.Post_App.ReEntry (arg, (ctxt, Phi_Sledgehammer_Solver.auto id ctxt sequent'))
+              in raise Phi_CP_IDE.Post_App.ReEntry (arg, (ctxt,
+                          Phi_Sledgehammer_Solver.auto id (Phi_Envir.freeze_dynamic_lemmas ctxt) sequent'))
               handle Phi_Reasoners.Automation_Fail err =>
                   error (Pretty.string_of (Pretty.chunks (err ())))
              end
@@ -2727,7 +2727,8 @@ in
             val b = if Binding.is_empty b'
                     then Binding.make (gen_name id', pos)
                     else b'
-            val (_,ctxt') = Proof_Context.add_fixes_cmd fixes ctxt
+            val ctxt' = Proof_Context.add_fixes_cmd fixes ctxt |> snd
+                     |> Phi_Envir.freeze_dynamic_lemmas
             val thms = map (Syntax.parse_prop ctxt') bodys'
                      |> Syntax.check_props ctxt'
                      |> map_index (fn (j,term) => term
