Phi_System/Phi_BI.thy
@@ -151,7 +151,7 @@ lemma \<phi>Type_protect_type_cong:
 \<Longrightarrow> x \<Ztypecolon> T \<equiv> x' \<Ztypecolon> T\<close>
   by simp
 
-setup \<open>Context.theory_map (PLPR_Rule_Gen.Template_Inst_SS.map (
+setup \<open>Context.theory_map (PLPR_Rule_Gen.Rule_Gen_SS.map (
   Simplifier.add_cong @{thm' \<phi>Type_protect_type_cong}))\<close>
 
 ML_file \<open>library/tools/simp_congruence.ML\<close>
